src/lowparse/pulse/LowParse.Pulse.Util.fst
@@ -53,7 +53,7 @@ fn slice_append_split (#t: Type) (mutb: bool) (s: S.slice t) (#p: perm) (#v1 #v2
 }
 ```
 
-let slice_append_split_stick_post'
+let slice_append_split_trade_post'
     (#t: Type) (s: S.slice t) (p: perm) (v1 v2: Ghost.erased (Seq.seq t)) (i: SZ.t)
     (s1: S.slice t)
     (s2: S.slice t)
@@ -63,16 +63,16 @@ let slice_append_split_stick_post'
             S.pts_to s2 #p v2 **
             (trade (S.pts_to s1 #p v1 ** S.pts_to s2 #p v2) (S.pts_to s #p (v1 `Seq.append` v2)))
 
-let slice_append_split_stick_post
+let slice_append_split_trade_post
     (#t: Type) (s: S.slice t) (p: perm) (v1 v2: Ghost.erased (Seq.seq t)) (i: SZ.t)
     (res: S.slice_pair t)
 : Tot vprop
 = let S.SlicePair s1 s2 = res in
-  slice_append_split_stick_post' s p v1 v2 i s1 s2
+  slice_append_split_trade_post' s p v1 v2 i s1 s2
 
 ```pulse
 ghost
-fn slice_append_split_stick_aux
+fn slice_append_split_trade_aux
   (#t: Type) (input: S.slice t) (p: perm) (v1 v2: (Seq.seq t)) (i: SZ.t) (input1 input2: S.slice t) (_: unit)
     requires S.is_split input p i input1 input2 ** (S.pts_to input1 #p v1 ** S.pts_to input2 #p v2)
     ensures S.pts_to input #p (v1 `Seq.append` v2)
@@ -84,26 +84,26 @@ fn slice_append_split_stick_aux
 inline_for_extraction
 noextract
 ```pulse
-fn slice_append_split_stick (#t: Type) (mutb: bool) (input: S.slice t) (#p: perm) (#v1 #v2: Ghost.erased (Seq.seq t)) (i: SZ.t)
+fn slice_append_split_trade (#t: Type) (mutb: bool) (input: S.slice t) (#p: perm) (#v1 #v2: Ghost.erased (Seq.seq t)) (i: SZ.t)
     requires S.pts_to input #p (v1 `Seq.append` v2) ** pure (slice_append_split_precond mutb p v1 i)
     returns res: S.slice_pair t
-    ensures slice_append_split_stick_post input p v1 v2 i res
+    ensures slice_append_split_trade_post input p v1 v2 i res
 {
   let res = slice_append_split mutb input i;
   match res {
     S.SlicePair input1 input2 -> {
       unfold (slice_append_split_post input p v1 v2 i res);
       unfold (slice_append_split_post' input p v1 v2 i input1 input2);
-      intro_trade _ _ _ (slice_append_split_stick_aux input p v1 v2 i input1 input2);
-      fold (slice_append_split_stick_post' input p v1 v2 i input1 input2);
-      fold (slice_append_split_stick_post input p v1 v2 i (S.SlicePair input1 input2));
+      intro_trade _ _ _ (slice_append_split_trade_aux input p v1 v2 i input1 input2);
+      fold (slice_append_split_trade_post' input p v1 v2 i input1 input2);
+      fold (slice_append_split_trade_post input p v1 v2 i (S.SlicePair input1 input2));
       (S.SlicePair input1 input2)
     }
   }
 }
 ```
 
-let slice_split_stick_post'
+let slice_split_trade_post'
     (#t: Type) (s: S.slice t) (p: perm) (v: Ghost.erased (Seq.seq t)) (i: SZ.t)
     (s1: S.slice t)
     (s2: S.slice t)
@@ -117,16 +117,16 @@ let slice_split_stick_post'
                 (v1, v2) == Seq.split v (SZ.v i)
             )
 
-let slice_split_stick_post
+let slice_split_trade_post
     (#t: Type) (s: S.slice t) (p: perm) (v: Ghost.erased (Seq.seq t)) (i: SZ.t)
     (res: S.slice_pair t)
 : Tot vprop
 = let (S.SlicePair s1 s2) = res in
-  slice_split_stick_post' s p v i s1 s2
+  slice_split_trade_post' s p v i s1 s2
 
 ```pulse
 ghost
-fn slice_split_stick_aux
+fn slice_split_trade_aux
   (#t: Type) (s: S.slice t) (p: perm) (v: Seq.seq t) (i: SZ.t)
   (s1 s2: S.slice t) (v1 v2: Seq.seq t) (hyp: squash (v == Seq.append v1 v2)) (_: unit)
     requires (S.is_split s p i s1 s2 ** (S.pts_to s1 #p v1 ** S.pts_to s2 #p v2))
@@ -139,10 +139,10 @@ fn slice_split_stick_aux
 inline_for_extraction
 noextract
 ```pulse
-fn slice_split_stick (#t: Type) (mutb: bool) (s: S.slice t) (#p: perm) (#v: Ghost.erased (Seq.seq t)) (i: SZ.t)
+fn slice_split_trade (#t: Type) (mutb: bool) (s: S.slice t) (#p: perm) (#v: Ghost.erased (Seq.seq t)) (i: SZ.t)
     requires S.pts_to s #p v ** pure (S.split_precond mutb p v i)
     returns res: S.slice_pair t
-    ensures slice_split_stick_post s p v i res
+    ensures slice_split_trade_post s p v i res
 {
   Seq.lemma_split v (SZ.v i);
   let res = S.split mutb s i;
@@ -150,9 +150,9 @@ fn slice_split_stick (#t: Type) (mutb: bool) (s: S.slice t) (#p: perm) (#v: Ghos
     unfold (S.split_post s p v i res);
     unfold (S.split_post' s p v i s1 s2);
     with v1 v2 . assert (S.pts_to s1 #p v1 ** S.pts_to s2 #p v2);
-    intro_trade _ _ _ (slice_split_stick_aux s p v i s1 s2 v1 v2 ());
-    fold (slice_split_stick_post' s p v i s1 s2);
-    fold (slice_split_stick_post s p v i (S.SlicePair s1 s2));
+    intro_trade _ _ _ (slice_split_trade_aux s p v i s1 s2 v1 v2 ());
+    fold (slice_split_trade_post' s p v i s1 s2);
+    fold (slice_split_trade_post s p v i (S.SlicePair s1 s2));
     (S.SlicePair s1 s2)
   }}
 }
